games/Obs.v
@@ -1,7 +1,6 @@
 Require Import ATS.
 Require Import KLR.
-
-
+Require Import Classical.
 
 Module Obs.
 
@@ -10,130 +9,146 @@ Module Obs.
   Section ATS.
     Context {GA GB : game} {S K} (α : ats GA GB S K).
 
-    Inductive reachable : relation S :=
-      | reachable_refl s mk :
+    Inductive state := st (mk : pmove GA GB * K) | div.
+
+    Inductive reachable : rel (option S) (option _) :=
+      | reachable_suspend s mk :
           ATS.suspend α s mk ->
-          reachable s s
+          reachable (Some s) (Some (st mk))
+      | reachable_none :
+          reachable None None
       | reachable_step s s' s'' :
           ATS.step α s s' ->
           reachable s' s'' ->
-          reachable s s''.
+          reachable (Some s) s''.
 
     CoInductive diverges (s : S) : Prop :=
       | forever_internal_intro s' :
-          ATS.step α s s' ->
+          ATS.step α s (Some s') ->
           diverges s' ->
           diverges s.
 
-    Inductive step : option S -> option S -> Prop :=
-      | step_intro : step None None.
+    Inductive step : state -> option state -> Prop :=
+      | step_intro : step div (Some div).
 
-    Inductive suspend : option S -> pmove GA GB * K -> Prop :=
-      | suspend_intro s mk :
-          ATS.suspend α s mk ->
-          suspend (Some s) mk.
+    Inductive suspend : state -> pmove GA GB * K -> Prop :=
+      | suspend_intro mk : suspend (st mk) mk.
 
-    Inductive resume : K -> omove GA GB -> option S -> Prop :=
+    Inductive resume : K -> omove GA GB -> option state -> Prop :=
       | resume_reachable k m s s' :
           ATS.resume α k m s ->
           reachable s s' ->
-          resume k m (Some s')
+          resume k m s'
       | resume_diverges k m s :
-          ATS.resume α k m s ->
+          ATS.resume α k m (Some s) ->
           diverges s ->
-          resume k m None.
+          resume k m (Some div).
 
     Definition of :=
-      ATS.Build_ats GA GB (option S) K step suspend resume (ATS.refuse α).
+      ATS.Build_ats GA GB state K step suspend resume (ATS.refuse α).
   End ATS.
+
+  Arguments state : clear implicits.
 
   (** ** Monotonicity *)
 
-  Global Instance reachable_sim :
-    Monotonic
-      (@reachable)
-      (forallr GRA, forallr GRB, forallr RS, forallr RK,
-       ATS.sim GRA GRB RS RK ++> |= RS ++> k1 set_le RS).
-  Proof.
-    intros GA1 GA2 GRA GB1 GB2 GRB S1 S2 RS K1 K2 RK α1 α2 Hα w.
-    intros s1 s2 Hs s1' Hs1'. revert s2 Hs.
-    induction Hs1' as [s1 mk1 H1 | s1 s1' s1'' Hs1' Hs1'' IHs1'']; intros.
-    - edestruct @ATS.sim_suspend as (mk2 & Hmk2 & Hmk); eauto.
-      eauto using reachable_refl.
-    - edestruct @ATS.sim_step as (s2' & Hs2' & Hs'); eauto.
-      edestruct IHs1'' as (s2'' & Hs2'' & Hs''); eauto.
-      eauto using reachable_step.
-  Qed.
+  Section SIM.
+    Context {GA1 GA2} (GRA : grel GA1 GA2).
+    Context {GB1 GB2} (GRB : grel GB1 GB2).
+    Context {S1 S2} (RS : klr (gworld GRA GRB) S1 S2).
+    Context {K1 K2} (RK : klr (gworld GRA GRB) K1 K2).
 
-  Global Instance diverges_sim :
-    Monotonic
-      (@diverges)
-      (forallr GRA, forallr GRB, forallr RS, forallr RK,
-       ATS.sim GRA GRB RS RK ++> |= RS ++> k impl).
-  Proof.
-    intros GA1 GA2 GRA GB1 GB2 GRB S1 S2 RS K1 K2 RK α1 α2 Hα w.
-    cofix IH.
-    intros s1 s2 Hs Hs1.
-    destruct Hs1 as [s1' Hs1' Hs1'd].
-    edestruct @ATS.sim_step as (s2' & Hs2' & Hs'); [ eauto .. | ].
-    econstructor; eauto.
-    eapply IH; eauto.
-  Qed.
+    Inductive state_rel : klr _ (state GA1 GB1 K1) (state GA2 GB2 K2) :=
+      | st_rel :
+          (|= (<> * RK) ++> state_rel)%rel st st
+      | div_rel :
+          (|= state_rel)%rel div div.
 
-  Global Instance step_sim :
-    Monotonic
-      (@step)
-      (forallr RS, option_rel RS ++> set_le (option_rel RS)).
-  Proof.
-    intros S1 S2 RS s1 s2 Hs s1' Hs1'.
-    destruct Hs1'; inversion Hs; subst.
-    exists None; repeat constructor.
-  Qed.
+    Lemma reachable_sim :
+      Monotonic reachable
+        (ATS.sim GRA GRB RS RK ++>
+         |= k1 option_ge RS ++> k1 set_le (k1 option_ge state_rel)).
+    Proof.
+      intros α1 α2 Hα w s1 s2 Hs s1' Hs1'. revert s2 Hs.
+      induction Hs1' as [s1 mk1 Hmk1 | | s1 s1' s1'' Hs1' Hs1'' IHs1'']; intros;
+      inversion Hs; clear Hs; subst;
+      try solve [exists None; repeat constructor; auto].
+      - edestruct @ATS.sim_suspend as (mk2 & Hmk2 & Hmk); eauto.
+        exists (Some (st mk2)). repeat constructor; auto.
+      - edestruct @ATS.sim_step as (s2' & Hs2' & Hs'); eauto.
+        edestruct IHs1'' as (s2'' & Hs2'' & Hs''); eauto.
+        exists s2''; split; auto.
+        eapply reachable_step; eauto.
+    Qed.
 
-  Global Instance suspend_sim :
-    Monotonic
-      (@suspend)
-      (forallr GRA, forallr GRB, forallr RS, forallr RK,
-       ATS.sim GRA GRB RS RK ++>
-       |= k1 option_rel RS ++> k1 set_le (<> * RK)).
-  Proof.
-    intros GA1 GA2 GRA GB1 GB2 GRB S1 S2 RS K1 K2 RK α1 α2 Hα w.
-    intros s1 s2 Hs mk1 Hmk1.
-    destruct Hmk1 as [s1 mk1 Hmk1]; inversion Hs; clear Hs; subst.
-    edestruct @ATS.sim_suspend as (mk2 & Hmk2 & Hmk); eauto.
-    exists mk2; intuition auto.
-    constructor; auto.
-  Qed.
+    Lemma diverges_sim α1 α2 w s1 s2 :
+      ATS.sim GRA GRB RS RK α1 α2 ->
+      RS w s1 s2 ->
+      diverges α1 s1 ->
+      diverges α2 s2 \/ reachable α2 (Some s2) None.
+    Proof.
+      intros Hα Hs Hs1.
+      destruct (classic (reachable α2 (Some s2) None)) as [ | Hsafe]; auto. left.
+      revert s1 s2 Hsafe Hs Hs1. cofix IH. intros.
+      destruct Hs1 as [s1' Hs1' Hs1'd].
+      edestruct @ATS.sim_step as (os2' & Hs2' & Hos'); [ eauto .. | ].
+      inversion Hos' as [xs1' s2' Hs' | xs1']; clear Hos'; subst.
+      - econstructor; eauto.
+        eapply IH; eauto.
+        intros Hs2'safe. apply Hsafe. econstructor; eauto.
+      - elim Hsafe. repeat econstructor; eauto.
+    Qed.
 
-  Global Instance resume_sim :
-    Monotonic
-      (@resume)
-      (forallr GRA, forallr GRB, forallr RS, forallr RK,
-       ATS.sim GRA GRB RS RK ++>
-       |= RK ++> [] -> k1 set_le (k1 option_rel RS)).
-  Proof.
-    intros GA1 GA2 GRA GB1 GB2 GRB S1 S2 RS K1 K2 RK α1 α2 Hα w.
-    intros k1 k2 Hk m1 m2 w' Hm s1 Hs1.
-    destruct Hs1 as [k1 m1 s1 s1' Hs1 Hs1' | k1 m1 s1 Hs1 Hd].
-    - edestruct @ATS.sim_resume as (s2 & Hs2 & Hs); eauto.
-      edestruct @reachable_sim as (s2' & Hs2' & Hs'); eauto.
-      exists (Some s2'); split.
-      + eauto using resume_reachable.
-      + rauto.
-    - edestruct @ATS.sim_resume as (s2 & Hs2 & Hs); eauto.
-      exists None; split.
-      + eapply resume_diverges; eauto.
-        eapply diverges_sim; eauto.
-      + rauto.
-  Qed.
+    Lemma step_sim :
+      Monotonic step (|= state_rel ++> k1 set_le (k1 option_ge state_rel)).
+    Proof.
+      intros w s1 s2 Hs s1' Hs1'.
+      destruct Hs1'; inversion Hs; subst.
+      exists (Some div); repeat constructor.
+    Qed.
+
+    Lemma suspend_sim :
+      Monotonic suspend (|= state_rel ++> k1 set_le (<> * RK)).
+    Proof.
+      intros w s1 s2 Hs mk1 Hmk1. destruct Hmk1 as [mk1].
+      inversion Hs as [xw xmk1 mk2 Hmk | ]; clear Hs; subst.
+      exists mk2; repeat constructor; auto.
+    Qed.
+
+    Lemma resume_sim :
+      Monotonic resume
+        (ATS.sim GRA GRB RS RK ++>
+         |= RK ++> [] -> k1 set_le (k1 option_ge state_rel)).
+    Proof.
+      intros α1 α2 Hα w k1 k2 Hk m1 m2 w' Hm s1 Hs1.
+      destruct Hs1 as [k1 m1 s1 s1' Hs1 Hs1' | k1 m1 s1 Hs1 Hd].
+      - edestruct @ATS.sim_resume as (s2 & Hs2 & Hs); eauto.
+        edestruct @reachable_sim as (s2' & Hs2' & Hs'); eauto.
+        exists s2'; split.
+        + eauto using resume_reachable.
+        + rauto.
+      - edestruct @ATS.sim_resume as (os2 & Hs2 & Hos); eauto.
+        inversion Hos as [xs1 s2 Hs | xs1]; clear Hos; subst.
+        + edestruct diverges_sim as [Hs2d | Hs2c]; eauto.
+          * exists (Some div). repeat constructor; auto.
+            eapply resume_diverges; eauto.
+          * exists None. repeat constructor; auto.
+            eapply resume_reachable; eauto.
+        + exists None. repeat constructor; auto.
+          eapply resume_reachable; eauto. constructor.
+    Qed.
+  End SIM.
 
   Global Instance of_sim :
     Monotonic
       (@of)
       (forallr GRA, forallr GRB, forallr RS, forallr RK,
-       ATS.sim GRA GRB RS RK ++> ATS.sim GRA GRB (k1 option_rel RS) RK).
+       ATS.sim GRA GRB RS RK ++> ATS.sim GRA GRB (state_rel GRA GRB RK) RK).
   Proof.
-    split; simpl; rauto.
+    split; simpl; repeat rstep.
+    - eapply step_sim; eauto.
+    - eapply suspend_sim; eauto.
+    - eapply resume_sim; eauto.
   Qed.
 
 End Obs.
